# Conditional rule
For some ***precondition*** $P$, ***side-effect free*** expression $E$, ***commands*** $S$ and $T$, and ***postcondition*** $Q$, we have the ***conditional rule***
$$\Large
\begin{gathered}
\large\begin{aligned}
&\textcolor{Cyan}{\text{// PRE:}} && P \\
&\textcolor{Lime}{\text{if ($E$) \{}} \\
&\textcolor{Cyan}{\ \ \ \ \ \ \ \ \text{// MID:}} && P \wedge E \\
&\textcolor{Lime}{\ \ \ \ \ \ \ \ S} \\
&\textcolor{Cyan}{\ \ \ \ \ \ \ \ \text{// MID:}} && Q \\
&\textcolor{Lime}{\text{\} else \{}} \\
&\textcolor{Cyan}{\ \ \ \ \ \ \ \ \text{// MID:}} && P \wedge \neg E \\
&\textcolor{Lime}{\ \ \ \ \ \ \ \ T} \\
&\textcolor{Cyan}{\ \ \ \ \ \ \ \ \text{// MID:}} && Q \\
&\textcolor{Lime}{\text{\}}} \\
&\textcolor{Cyan}{\text{// POST:}} && Q \\
\end{aligned} && \iff &&
\begin{prooftree}  
\AxiomC{$\{ P \wedge E \} \ \textcolor{Lime}{S} \ \{ Q \}$}
\AxiomC{$\{ P \wedge \neg E \} \ \textcolor{Lime}{T} \ \{ Q \}$}
\BinaryInfC{$\{ P \} \ \textcolor{Lime}{\text{if ($E$) \{ $S$ \} else \{ $T$} \}} \ \{ Q \}$}  
\end{prooftree}
\end{gathered}
$$
Which states that if ***postcondition*** $Q$ common to *both* conditional branches, then it is ***also*** the postcondition of to *entire* conditional statement.

## Conditional rule in practice 
While the [[#Conditional rule|conditional rule]] boils down the essence of conditional branching, it is not as useful as it could be. This is because, we will almost never be able to arrive at the same ***postcondition*** in both branches *"for free"*. Instead we will have something like this:
$$\large
\begin{leftalign}
&\textcolor{Cyan}{\text{// PRE:}} && P \\
&\textcolor{Lime}{\text{if ($E$) \{}} \\
&\textcolor{Cyan}{\ \ \ \ \ \ \ \ \text{// MID:}} && P \wedge E \\
&\textcolor{Lime}{\ \ \ \ \ \ \ \ S} \\
&\textcolor{Cyan}{\ \ \ \ \ \ \ \ \text{// MID:}} && \textcolor{Red}{R_{1}} \\
&\textcolor{Lime}{\text{\} else \{}} \\
&\textcolor{Cyan}{\ \ \ \ \ \ \ \ \text{// MID:}} && P \wedge \neg E \\
&\textcolor{Lime}{\ \ \ \ \ \ \ \ T} \\
&\textcolor{Cyan}{\ \ \ \ \ \ \ \ \text{// MID:}} && \textcolor{Red}{R_{2}} \\
&\textcolor{Lime}{\text{\}}} \\
\end{leftalign}
$$
The two branches have ***postconditions*** $R_{1}$ and $R_{2}$, respectively. We can employ the [[5. Kotlin - Specifying Programs#Consequence rule|consequence rule]] to ***weaken*** them both to $Q$ by meeting the following proof obligations
$$\large \textcolor{Red}{R_{1}} \to Q \ \ \ \ \wedge \ \ \ \ \textcolor{Red}{R_{2}} \to Q$$
Which, put altogether, becomes the <b><u>practical</u></b> [[#Conditional rule|conditional rule]]
$$\Large
\begin{gathered}
\large\begin{aligned}
&\textcolor{Cyan}{\text{// PRE:}} && P \\
&\textcolor{Lime}{\text{if ($E$) \{}} \\
&\textcolor{Cyan}{\ \ \ \ \ \ \ \ \text{// MID:}} && P \wedge E \\
&\textcolor{Lime}{\ \ \ \ \ \ \ \ S} \\
&\textcolor{Cyan}{\ \ \ \ \ \ \ \ \text{// MID:}} && \textcolor{Red}{R_{1}} \\
&\textcolor{Lime}{\text{\} else \{}} \\
&\textcolor{Cyan}{\ \ \ \ \ \ \ \ \text{// MID:}} && P \wedge \neg E \\
&\textcolor{Lime}{\ \ \ \ \ \ \ \ T} \\
&\textcolor{Cyan}{\ \ \ \ \ \ \ \ \text{// MID:}} && \textcolor{Red}{R_{2}} \\
&\textcolor{Lime}{\text{\}}} \\
&\textcolor{Cyan}{\text{// POST:}} && Q \\
\end{aligned} && \iff &&
\begin{prooftree}
\AxiomC{$\textcolor{Red}{R_{1}} \to Q \wedge \textcolor{Red}{R_{2}} \to Q$}
\AxiomC{$\{ P \wedge E \} \ \textcolor{Lime}{S} \ \{ \textcolor{Red}{R_{1}} \}$}
\AxiomC{$\{ P \wedge \neg E \} \ \textcolor{Lime}{T} \ \{ \textcolor{Red}{R_{2}} \}$}
\TrinaryInfC{$\{ P \} \ \textcolor{Lime}{\text{if ($E$) \{ $S$ \} else \{ $T$} \}} \ \{ Q \}$}  
\end{prooftree}
\end{gathered}
$$

# Example
![[Pasted image 20240417194657.png|800]]
![[Pasted image 20240417194713.png|800]]
![[Pasted image 20240417194553.png|800]]
![[Pasted image 20240417194745.png|800]]
